CertiGC/verif_forward.v
@@ -1,21 +1,41 @@
 Require Import RamifyCoq.CertiGC.gc_spec.
 
-Lemma root_valid_int_or_ptr: forall g (roots: roots_t) root,
+
+Lemma root_valid_int_or_ptr: forall g (roots: roots_t) root outlier,
     In root roots ->
-    Forall (graph_has_v g) (filter_sum_right roots) ->
-    graph_rep g |-- !! (valid_int_or_ptr (root2val g root)).
+    roots_compatible g outlier roots ->
+    graph_rep g * outlier_rep outlier |-- !! (valid_int_or_ptr (root2val g root)).
 Proof.
-  intros. destruct root as [[? | ?] | ?].
+  intros. destruct H0. destruct root as [[? | ?] | ?].
   - simpl root2val. unfold odd_Z2val. replace (2 * z + 1) with (z + z + 1) by omega.
     apply prop_right, valid_int_or_ptr_ii1.
-  - destruct g0. simpl. inv_int i. rewrite ptrofs_add_repr.
-    replace (ofs + ofs) with (2 * ofs)%Z by omega. apply prop_right.
-    rewrite Ptrofs.unsigned_repr_eq, Zodd_mod, <- Zmod_div_mod; try rep_omega.
-    + rewrite Z.mul_comm, Z_mod_mult. unfold Zeq_bool. reflexivity.
-    + exists (Z.div Ptrofs.modulus 2). reflexivity.
-  - rewrite Forall_forall in H0. rewrite (filter_sum_right_In_iff v roots) in H.
-    apply H0 in H. simpl. apply graph_rep_valid_int_or_ptr. assumption.
+  - sep_apply (outlier_rep_single_rep _ _ _ H H0).
+    sep_apply (single_outlier_rep_valid_int_or_ptr g0). entailer!.
+  - rewrite Forall_forall in H1. rewrite (filter_sum_right_In_iff v roots) in H.
+    apply H1 in H. simpl. sep_apply (graph_rep_valid_int_or_ptr _ _ H). entailer!.
 Qed.
+
+Lemma single_outlier_rep_memory_block_FF: forall gp p n wsh,
+    writable_share wsh -> v_in_range (GC_Pointer2val gp) p (WORD_SIZE * n) ->
+    single_outlier_rep gp * data_at_ wsh (tarray int_or_ptr_type n) p |-- FF.
+Proof.
+  intros. unfold single_outlier_rep. Intros rsh. remember (GC_Pointer2val gp) as ggp.
+  clear gp Heqggp. rename ggp into gp. destruct H0 as [o [? ?]].
+  rewrite !data_at__memory_block. Intros. clear H3. destruct H4 as [? [_ [? _]]].
+  destruct p; try contradiction. subst gp. inv_int i. simpl offset_val.
+  assert (0 <= n) by rep_omega. rewrite ptrofs_add_repr.
+  rewrite sizeof_tarray_int_or_ptr by assumption. simpl sizeof. simpl in H4.
+  rewrite Ptrofs.unsigned_repr in H4 by rep_omega. rewrite Z.max_r in H4 by assumption.
+  rewrite WORD_SIZE_eq in *. rewrite sepcon_assoc, (sepcon_comm TT), <- sepcon_assoc.
+  assert (4 * n = o + (4 * n - o))%Z by omega. remember (4 * n - o) as m.
+  rewrite H6 in *. rewrite (memory_block_split wsh b ofs o m) by omega.
+  clear Heqm n H6 H2. assert (0 < m <= Ptrofs.max_unsigned) by rep_omega.
+  assert (0 < 4 <= Ptrofs.max_unsigned) by rep_omega.
+  rewrite (sepcon_comm (memory_block wsh o (Vptr b (Ptrofs.repr ofs)))),
+  <- sepcon_assoc. remember (Vptr b (Ptrofs.repr (ofs + o))) as p.
+
+  (* memory_block_conflict *)
+Admitted.
 
 Lemma body_forward: semax_body Vprog Gprog f_forward forward_spec.
 Proof.
@@ -39,42 +59,47 @@ Proof.
         simpl. exact I.
     } forward. 1: apply prop_right, (fi_index_range f_info), Znth_In; assumption.
     1: entailer!; rewrite H7; assumption. rewrite H7.
-    destruct H4. sep_apply (root_valid_int_or_ptr g roots root H8 H10). Intros.
-    forward_call (root2val g root). destruct root as [[? | ?] | ?]; simpl root2val.
+    assert_PROP (valid_int_or_ptr (root2val g root)). {
+      gather_SEP 3 2. sep_apply (root_valid_int_or_ptr _ _ _ _ H8 H4). entailer!.
+    } forward_call (root2val g root). destruct root as [[? | ?] | ?]; simpl root2val.
     + unfold odd_Z2val. forward_if True.
-      1: exfalso; apply H12'. reflexivity. 1: forward; entailer!.
+      1: exfalso; apply H11'. reflexivity. 1: forward; entailer!.
       forward. Exists g t_info roots. entailer!.
       * unfold roots_compatible. intuition. rewrite <- Heqroot. simpl. constructor.
       * unfold thread_info_rep. entailer!.
     + unfold GC_Pointer2val. destruct g0. forward_if True.
-      2: exfalso; apply Int.one_not_zero in H12; assumption.
-      * forward_call (Vptr b (Ptrofs.add i i)).
-        gather_SEP 0 6 3. rewrite <- sepcon_assoc.
+      2: exfalso; apply Int.one_not_zero in H11; assumption.
+      * forward_call (Vptr b i). gather_SEP 3 6 2. rewrite <- sepcon_assoc.
         remember (graph_rep g * heap_rest_rep (ti_heap t_info) * outlier_rep outlier)
-          as P.
-        pose proof (outlier_rep_valid_pointer roots outlier (GCPtr b i) H8 H4).
-        pose proof (graph_and_heap_rest_memory_block _ _ _ H1 H).
+          as P. destruct H4. pose proof (graph_and_heap_rest_data_at_ _ _ _ H1 H).
         remember (nth_gen g from).(generation_sh) as fsh.
-        remember (gen_start g from) as fp.
-        remember (WORD_SIZE * gen_size t_info from)%Z as fn.
+        remember (gen_start g from) as fp. remember (gen_size t_info from) as gn.
+        remember (WORD_SIZE * gn)%Z as fn.
         assert (P |-- (weak_derives P (memory_block fsh fn fp * TT) && emp) * P). {
           subst. cancel. apply andp_right. 2: cancel.
           assert (HS: emp |-- TT) by entailer; sep_apply HS; clear HS.
-          apply derives_weak. sep_apply H14. cancel.
+          apply derives_weak. sep_apply H13. rewrite data_at__memory_block.
+          rewrite sizeof_tarray_int_or_ptr; [Intros; cancel | unfold gen_size].
+          destruct (total_space_tight_range (nth_space t_info from)). assumption.
         } replace_SEP 0 ((weak_derives P (memory_block fsh fn fp * TT) && emp) * P) by
-            (entailer; assumption). clear H15. Intros. simpl root2val in *.
-        assert (P |-- (weak_derives P (valid_pointer (Vptr b (Ptrofs.add i i)) * TT) &&
-                                    emp) * P). {
+            (entailer; assumption). clear H14. Intros. simpl root2val in *.
+        assert (P |-- (weak_derives P (valid_pointer (Vptr b i) * TT) && emp) * P). {
           subst. cancel. apply andp_right. 2: cancel.
           assert (HS: emp |-- TT) by entailer; sep_apply HS; clear HS.
-          apply derives_weak. sep_apply H13. simpl GC_Pointer2val. cancel. }
-        replace_SEP
-        1 ((weak_derives P (valid_pointer (Vptr b (Ptrofs.add i i)) * TT) &&
-                         emp) * P) by (entailer; assumption). Intros. clear H15.
-        forward_call (fsh, fp, fn, (Vptr b (Ptrofs.add i i)), P). Intros v. destruct v.
-        -- subst P. Intros. gather_SEP 0 1. sep_apply H14. sep_apply H13. Intros.
-           simpl GC_Pointer2val. gather_SEP 0 2. admit.
-        -- forward_if. 1: exfalso; apply H15'; reflexivity. forward. entailer!.
+          apply derives_weak.
+          sep_apply (outlier_rep_valid_pointer roots outlier (GCPtr b i) H8 H4).
+          simpl GC_Pointer2val. cancel. }
+        replace_SEP 1 ((weak_derives P (valid_pointer (Vptr b i) * TT) && emp) * P) by
+            (entailer; assumption). Intros. clear H14.
+        forward_call (fsh, fp, fn, (Vptr b i), P). Intros v. destruct v.
+        -- rewrite HeqP. Intros. gather_SEP 0 1. sep_apply H13. rewrite Heqfn in v.
+           sep_apply (outlier_rep_single_rep _ _ _ H8 H4). Intros. gather_SEP 0 2.
+           change (Vptr b i) with (GC_Pointer2val (GCPtr b i)) in v.
+           pose proof (generation_share_writable (nth_gen g from)).
+           rewrite <- Heqfsh in H14.
+           sep_apply (single_outlier_rep_memory_block_FF (GCPtr b i) fp gn fsh H14 v).
+           assert_PROP False by entailer!. contradiction.
+        -- forward_if. 1: exfalso; apply H14'; reflexivity. forward. entailer!.
       * forward. Exists g t_info roots. entailer!.
         -- unfold roots_compatible. intuition. rewrite <- Heqroot. simpl. constructor.
         -- unfold thread_info_rep. entailer!.
