CertiGC/verif_resume.v
@@ -74,7 +74,7 @@ Proof.
       unfold space_rest_rep at 1. rewrite <- H3, <- H4, if_false. 2: discriminate.
       freeze [1; 2; 3; 4; 5] FR. gather_SEP 1 2.
       assert (0 <= used_space hs <= total_space hs) by (apply space_order).
-      sep_apply (data_at__tarray_value_join
+      sep_apply (data_at__tarray_value_fold
                    sh0 (total_space hs) (used_space hs) (Vptr b i) H8). thaw FR.
       forward. Exists (reset_nth_gen_graph O g) (reset_nth_heap_thread_info O t_info).
       entailer!.
